compiler/dsl/coq/ReflexEcho.v
@@ -3,6 +3,8 @@ Require Import String.
 Require Import Reflex.
 Require Import ReflexBase.
 Require Import ReflexDenoted.
+Require Import ReflexFin.
+Require Import ReflexFrontend.
 Require Import ReflexVec.
 
 Open Scope string_scope.
@@ -26,25 +28,21 @@ Definition COMPS (t : COMPT) : comp :=
   | Echo => mk_comp "Echo" "test/echo-00/test.py" []
   end.
 
-Definition INIT : init_prog PAYD COMPT KSTD IENVD :=
-  [fun s => Spawn _ _ _ IENVD Echo None (Logic.eq_refl _)
+Definition INIT : init_prog PAYD COMPT KSTD (init_msg PAYD) IENVD :=
+  [fun s => Spawn _ _ _ _ IENVD Echo None (Logic.eq_refl _)
   ].
 
 Definition HANDLERS : handlers PAYD COMPT KSTD :=
-  (fun m cfd =>
-    match tag PAYD m as _tm return
-      @sdenote _ SDenoted_vdesc (lkup_tag PAYD _tm) -> _
-    with
-    | None => fun pl =>
-       let envd := existT _ 0 tt in
-       existT (fun d => hdlr_prog PAYD COMPT KSTD d) envd (
-         let (msg, _) := pl in fun st0 =>
-         [ fun s => Send PAYD _ _ _ (CFd _ _) None (SLit _ _ msg, tt)
-         ]
-       )
-    | Some bad => fun _ =>
+  fun (m : msg PAYD) cfd =>
+    match m as _m return forall (EQ : _m = m), _ with
+    | Build_msg None p => fun EQ =>
+      let envd := existT _ 0 tt in
+      existT (fun d => hdlr_prog PAYD COMPT KSTD _ d) envd (
+        let (msg, _) := p in fun st0 =>
+        [ fun s => Send _ _ _ _ _ (CFd PAYD _ _ _) None (mvar EQ None, tt) ]
+      )
+    | Build_msg (Some bad) _ =>
       match bad with end
-    end (pay PAYD m)
-  ).
+    end (Logic.eq_refl m).
 
 Definition main := mk_main (Build_spec NB_MSG PAYD IENVD KSTD COMPT COMPS INIT HANDLERS).
