compiler/dsl/coq/ReflexFrontend.v
@@ -1,0 +1,54 @@
+Require Import String.
+
+Require Import Reflex.
+Require Import ReflexBase.
+
+Record spec :=
+{ NB_MSG   : nat
+; PAYD     : vvdesc NB_MSG
+; IENVD    : vdesc
+; KSTD     : vdesc
+; COMPT    : Type
+; COMPS    : COMPT -> comp
+; INIT     : init_prog PAYD COMPT KSTD (init_msg PAYD) IENVD
+; HANDLERS : handlers PAYD COMPT KSTD
+}.
+
+Definition mk_main (s : spec) :=
+  @main _ (PAYD s) (COMPT s) (COMPS s) (KSTD s) (IENVD s) (INIT s) (HANDLERS s).
+
+Fixpoint mk_vdesc' l : vdesc' (List.length l) :=
+  match l with
+  | nil     => tt
+  | x :: xs => (x, mk_vdesc' xs)
+  end.
+
+Definition mk_vdesc l : vdesc := existT _ (List.length l) (mk_vdesc' l).
+
+Fixpoint mk_vvdesc (l : list (string * list desc)) : vvdesc (List.length l) :=
+  match l with
+  | nil          => tt
+  | (_, x) :: xs => (mk_vdesc x, mk_vvdesc xs)
+  end.
+
+Definition mk_comp name cmd args :=
+  {| comp_name := str_of_string name
+   ; comp_cmd  := str_of_string cmd
+   ; comp_args := List.map str_of_string args
+   |}.
+
+Notation " [ ] " := nil.
+Notation " [ x ] " := (cons x nil).
+Notation " [ x ; .. ; y ] " := (cons x .. (cons y nil) ..).
+
+Definition cast_m_expr {NB_MSG} {PAYD : vvdesc NB_MSG} {KSTD envd} {m : msg PAYD} {t p d}
+  (EQ : Build_msg PAYD t p = m) (e : expr PAYD KSTD (Build_msg PAYD t p) envd d)
+  : expr PAYD KSTD m envd d
+  :=
+  match EQ in _ = _m return expr _ _ _m _ _ with
+  | Logic.eq_refl => e
+  end.
+
+Definition mvar {NB_MSG} {PAYD : vvdesc NB_MSG} {KSTD envd} {m : msg PAYD} {t p}
+  (EQ : Build_msg PAYD t p = m) i :=
+  cast_m_expr EQ (MVar PAYD KSTD (Build_msg PAYD t p) envd i).
